AwsCryptographicMaterialProviders/dafny/AwsCryptographyKeyStoreAdmin/test/TestMutateToHV2FromHV1.dfy
@@ -15,7 +15,7 @@ module {:options "/functionSyntax:4" } TestMutateToHV2FromHV1 {
   import Types = AwsCryptographyKeyStoreAdminTypes
   import KeyStoreTypes = AwsCryptographyKeyStoreTypes
 
-  const testMutateForHV2ErrorsForNotKMSSimple := "dafny-initialize-mutation-hv-2-allowed"
+  const testMutateForHV2ErrorsForNotKMSSimple := "dafny-initialize-mutation-hv-2-bad-strategy"
   method {:test} TestMutateForHV2ErrorsForNotKMSSimple()
   {
     var uuid :- expect UUID.GenerateUUID();
@@ -40,8 +40,35 @@ module {:options "/functionSyntax:4" } TestMutateToHV2FromHV1 {
     var initializeOutput := underTest.InitializeMutation(initInput);
     var _ := CleanupItems.DeleteBranchKey(Identifier:=testId, ddbClient:=ddbClient);
     expect initializeOutput.Failure?, "Should have failed to InitializeMutation HV-2.";
-    expect initializeOutput.error.KeyStoreAdminException?;
+    expect initializeOutput.error.UnsupportedFeatureException?;
     // TODO-HV-2-M4: Support other key strategy as well.
-    expect initializeOutput.error.message == "Only KeyManagementStrategy.AwsKmsSimple is allowed when mutating to hv-2.", "Incorrect error message. Should have had `Only KeyManagementStrategy.AwsKmsSimple is allowed when mutating to hv-2.`";
+    expect initializeOutput.error.message == "Unsupported KeyManagementStrategy. Only KeyManagementStrategy.AwsKmsReEncrypt and KeyManagementStrategy.AwsKmsDecryptEncrypt is allowed when terminal hierarchical version is 1. Only KeyManagementStrategy.kmsSimple is allowed when terminal hierarchical version is 2.", "Incorrect error message. Should have had `Only KeyManagementStrategy.AwsKmsSimple is allowed when mutating to hv-2.`";
+  }
+
+  const testMutateForHV2SucceedsForKMSSimple := "dafny-initialize-mutation-hv-2-allowed"
+  method {:test} TestMutateForHV2SucceedsForKMSSimple()
+  {
+    var uuid :- expect UUID.GenerateUUID();
+    var testId := testMutateForHV2SucceedsForKMSSimple + "-" + uuid;
+    var ddbClient :- expect Fixtures.ProvideDDBClient();
+    var kmsClient :- expect Fixtures.ProvideKMSClient();
+    var underTest :- expect AdminFixtures.DefaultAdmin(ddbClient?:=Some(ddbClient));
+    var strategy :- expect AdminFixtures.SimpleKeyManagerStrategy(kmsClient?:=Some(kmsClient));
+    var systemKey := Types.SystemKey.trustStorage(trustStorage := Types.TrustStorage());
+    Fixtures.CreateHappyCaseId(id:=testId);
+
+    var mutationsRequest := Types.Mutations(
+      TerminalKmsArn := Some(Fixtures.postalHornKeyArn),
+      TerminalHierarchyVersion := Some(KeyStoreTypes.HierarchyVersion.v2)
+    );
+    var initInput := Types.InitializeMutationInput(
+      Identifier := testId,
+      Mutations := mutationsRequest,
+      Strategy := Some(strategy),
+      SystemKey := systemKey,
+      DoNotVersion := Some(true));
+    var initializeOutput := underTest.InitializeMutation(initInput);
+    var _ := CleanupItems.DeleteBranchKey(Identifier:=testId, ddbClient:=ddbClient);
+    expect initializeOutput.Success?, "Should have succeeded to InitializeMutation HV-2 for HV-2";
   }
 }
